Improve Hex.lean

Clvm/Hex.lean
@@ -1,4 +1,5 @@
-import Clvm.Result
+import Mathlib.Tactic.ByContra
+import Mathlib.Tactic.Use
 
 
 def hex_nibble_to_byte (c: Char) : Result Nat Char :=
@@ -11,29 +12,41 @@ def hex_nibble_to_byte (c: Char) : Result Nat Char :=
     Result.err c "invalid hex digit"
 
 
-def list_char_2b (s: List Char) : Result (List Nat) (List Char) :=
+def hex_pair_to_byte (c1 c2: Char) : Result Nat Char :=
+  match hex_nibble_to_byte c1, hex_nibble_to_byte c2 with
+  | Result.ok c1, Result.ok c2 => Result.ok (c1 * 16 + c2)
+  | Result.err c1 m1, _ => Result.err c1 m1
+  | _, Result.err c2 m2 => Result.err c2 m2
+
+
+def h2b_lc (s: List Char) : Result (List Nat) (List Char) :=
   match s with
   | c1 :: c2 :: rest =>
-    match hex_nibble_to_byte c1, hex_nibble_to_byte c2, list_char_2b rest with
-    | Result.ok c1, Result.ok c2, Result.ok r => Result.ok ((c1 * 16 + c2) :: r)
-    | Result.err c e, _, _ => Result.err [c] e
-    | _, Result.err c e, _ => Result.err [c] e
-    | _, _, Result.err c e => Result.err c e
+    match hex_pair_to_byte c1 c2, h2b_lc rest with
+    | Result.ok b, Result.ok r => Result.ok (b :: r)
+    | Result.err c e, _ => Result.err [c] e
+    | _, Result.err cs e => Result.err cs e
   | [c] => Result.err [c] "odd number of hex digits"
   | [] => Result.ok []
 
 
-def h2b_list (s: String) : Result (List Nat) String :=
-  match list_char_2b s.data with
+def h2b_lc! (s: List Char) : List Nat :=
+  match h2b_lc s with
+  | Result.ok r => r
+  | Result.err _ _ => []
+
+
+@[simp]
+def h2b (s: String) : Result (List Nat) String :=
+  match h2b_lc s.data with
   | Result.ok r => Result.ok r
   | Result.err c e => Result.err (String.mk c) e
 
 
-@[simp]
-def h2b (s: String) : Result (Array Nat) String :=
-  match (h2b_list s) with
-  | Result.ok r => Result.ok r.toArray
-  | Result.err _ e => Result.err s e
+def h2b! (s: String) : List Nat :=
+  match h2b s with
+  | Result.ok r => r
+  | Result.err _ _ => []
 
 
 
@@ -54,3 +67,91 @@ def b2h_uint8 (bytes : List UInt8) : String :=
 
 def List.hex (bytes: List Nat) : String :=
   b2h bytes
+
+
+theorem h2b_lc_remove_two_chars_helper: is_ok (h2b_lc ([c0, c1] ++ s)) →
+    is_ok (hex_pair_to_byte c0 c1) ∧ is_ok (h2b_lc s) := by
+  intro h
+  obtain ⟨ns, h0⟩ := h
+  unfold h2b_lc at h0
+  simp at h0
+  have p0: is_ok (hex_pair_to_byte c0 c1) := by
+    by_contra h1
+    obtain ⟨c, s0, h2⟩ := not_ok h1
+    simp [h2] at h0
+  simp [p0]
+  obtain ⟨n0, hn0⟩ := p0
+  rw [hn0] at h0
+  have p1: is_ok (h2b_lc s) := by
+    by_contra h1
+    obtain ⟨c, s0, h2⟩ := not_ok h1
+    simp [h2] at h0
+  exact p1
+
+
+theorem h2b_lc_remove_two_chars: is_ok (h2b_lc ([c0, c1] ++ s)) → h2b_lc ([c0, c1] ++ s) = Result.ok (h2b_lc! ([c0, c1]) ++ h2b_lc! s) := by
+  intro h0
+  obtain ⟨ p0, p1 ⟩ := h2b_lc_remove_two_chars_helper h0
+  obtain ⟨ns0, hn0⟩ := p0
+  obtain ⟨ns1, hn1⟩ := p1
+  simp [h2b_lc, h2b_lc!, hn0, hn1, h2b_lc]
+
+
+theorem take_drop (s : List α) (n: Nat): s = (s.take n) ++ (s.drop n) := by simp [List.take, List.drop]
+
+
+theorem prefix_len_2 (s: List α) : s.length ≥ 2 → ∃ c0 c1 r, s = [c0, c1] ++ r := by
+  intro h_len
+  cases s with
+  | nil => simp at h_len
+  | cons c0 s0 =>
+    cases s0 with
+    | nil => simp at h_len
+    | cons c1 s1 => simp [List.length] at h_len ; simp
+
+
+theorem h2b_lc_take_drop: is_ok (h2b_lc s) → s.length ≥ 2 → h2b_lc s = Result.ok (h2b_lc! (s.take 2) ++ h2b_lc! (s.drop 2)) := by
+  intro h0
+  intro h_len
+
+  obtain ⟨c0, c1, r, h2⟩ := prefix_len_2 s h_len
+  rw [h2] at h0
+  rw [h2]
+  rw [(h2b_lc_remove_two_chars h0)]
+  simp
+
+
+theorem h2b_lc_ok : is_ok (h2b s) → is_ok (h2b_lc s.data) := by
+  intro h
+  by_contra h1
+  obtain ⟨c, s0, h2⟩ := not_ok h1
+  simp [h2, is_ok] at h
+
+
+theorem h2b_eq_lc : is_ok (h2b s) → h2b! s = h2b_lc! s.data := by
+  intro h
+  obtain ⟨ns, h1⟩ := h2b_lc_ok h
+  simp [h2b_lc!, h2b!, h2b, h1]
+
+
+theorem h2b_eq_! : is_ok (h2b s) → h2b s = Result.ok (h2b! s) := by
+  intro h
+  obtain ⟨ns, h1⟩ := h2b_lc_ok h
+  simp [h2b_lc!, h2b!, h2b, h1]
+
+
+theorem h2b_lc_eq_! : is_ok (h2b s) → h2b_lc s.data = Result.ok (h2b_lc! s.data) := by
+  intro h
+  obtain ⟨ns, h1⟩ := h2b_lc_ok h
+  simp [h2b_lc!, h2b!, h2b, h1]
+
+
+theorem h2b_ok_iff_h2b_lc_ok : is_ok (h2b s) ↔ is_ok (h2b_lc s.data) := by
+  constructor
+  intro h
+  simp [(h2b_lc_eq_! h), is_ok]
+  intro h
+  simp [h2b]
+  obtain ⟨ns, h1⟩ := h
+  rw [h1]
+  simp [is_ok]
